Move from lists to pairs

src/CEK.v
@@ -4,6 +4,7 @@ Require Export
   Sub
   Sem
   Eval
+  Norm
   Coq.micromega.Lia.
 
 From Equations Require Import Equations.
@@ -16,8 +17,11 @@ Import ListNotations.
 Section CEK.
 
 Inductive Value : Ty → Type :=
-  | VLit {ty} : Literal ty → Value (TyPrim ty)
-  | VList {τ} : list (Value τ) → Value (TyList τ)
+  | VConst {ty}        : Literal ty → Value (TyPrim ty)
+  | VUnit              : Value TyUnit
+  | VTrue              : Value TyBool
+  | VFalse             : Value TyBool
+  | VPair {τ1 τ2}      : Value τ1 → Value τ2 → Value (TyPair τ1 τ2)
   | VClosure {dom cod} : Closure dom cod → Value (dom ⟶ cod)
 
 with Closure : Ty → Ty → Type :=
@@ -27,30 +31,36 @@ with Env : Env → Type :=
   | Empty : Env []
   | Val {Γ τ} : Value τ → Env Γ → Env (τ :: Γ).
 
-Derive Signature NoConfusion Subterm for Value.
+Derive Signature NoConfusion for Value.
 Derive Signature NoConfusion Subterm for Closure.
 Derive Signature NoConfusion for Env.
+
+Inductive represents Γ : ∀ {τ}, Exp Γ τ → Value τ → Prop :=
+  | VConst_represents {ty} (l : Literal ty) :
+    represents Γ (Constant l) (VConst l)
+  | VUnit_represents  : represents Γ EUnit VUnit
+  | VTrue_represents  : represents Γ ETrue VTrue
+  | VFalse_represents : represents Γ EFalse VFalse
+  | VPair_represents {τ1 τ2} (x : Exp Γ τ1) x' (y : Exp Γ τ2) y' :
+    represents Γ x x' →
+    represents Γ y y' →
+    represents Γ (Pair x y) (VPair x' y')
+  | VClosure_represents {dom cod} (e : Exp (dom :: Γ) cod) (ρ : Env Γ) :
+    represents Γ (LAM e) (VClosure (Lambda e ρ)).
+
+Lemma represents_values Γ {τ : Ty} (v : Exp Γ τ) (v' : Value τ) :
+  represents Γ v v' → ValueP v.
+Proof.
+  intros.
+  now induction H; constructor.
+Qed.
 
 Equations get `(se : Env Γ) `(v : Var Γ τ) : Value τ :=
   get (Val x _)   ZV    := x;
   get (Val _ xs) (SV v) := get xs v.
 
-(* Although this type is structurally equivalent to [option (list a)], the
-   type indices allow us to prevent it from being passed to [MkΣ] unless its
-   expression argument is of type [TyLList]. *)
-Inductive Accum Γ : ∀ τ : Ty, Exp Γ τ → Type :=
-  | ANone {τ e} : Accum Γ τ e
-  | AList {τ l} : list (Value τ) → Accum Γ (TyList τ) (List l).
-
-Arguments ANone {Γ τ e}.
-Arguments AList {Γ τ l} _.
-
-Derive Signature NoConfusion Subterm for Accum.
-
 Inductive Kont : Ty → Ty → Type :=
-  | Mt {a} : Kont a a
-  | Ar {Γ a b c} : Exp Γ a → Env Γ → Kont b c → Kont (a ⟶ b) c
-  | Fn {a b} : (Value a → Σ b) → Kont a b
+  | Fn {a b} : (Value a → Σ b + Value b) → Kont a b
 
 with Σ : Ty → Type :=
   | MkΣ (τ   : Ty)
@@ -58,10 +68,9 @@ with Σ : Ty → Type :=
         (r   : Ty)
         (exp : Exp Γ r)
         (env : Env Γ)
-        (acc : Accum Γ r exp)
         (knt : Kont r τ) : Σ τ.
 
-Derive Signature NoConfusion for Kont.
+Derive Signature NoConfusion Subterm for Kont.
 Derive Signature NoConfusion Subterm for Σ.
 
 Arguments MkΣ {τ Γ r} _ _ _.
@@ -70,118 +79,132 @@ Arguments MkΣ {τ Γ r} _ _ _.
    results of the evaluation. Therefore, the resulting [env] will be a
    singleton list containing that value. *)
 Definition inject {τ : Ty} {Γ : Exp.Env} (e : Exp Γ τ) (E : Env Γ) : Σ τ :=
-  MkΣ e E ANone Mt.
+  MkΣ e E (Fn inr).
 
-Equations step {τ : Ty} (s : Σ τ) : Σ τ :=
-  (* A constant is passed as a literal *)
-  step (MkΣ (Constant x) _ ANone (Fn f)) :=
-    f (VLit x);
+Equations IfBody {τ : Ty} {Γ : Exp.Env} (t e : Exp Γ τ)
+          (v : Value TyBool) : Exp Γ τ :=
+  IfBody t _ VTrue  := t;
+  IfBody _ e VFalse := e.
 
-  (* Lists are evaluated step-wise using Ls *)
-  step (MkΣ (List []) ρ ANone (Fn f)) :=
-    f (VList []);
-  step (MkΣ (List []) ρ (AList r) (Fn f)) :=
-    f (VList (rev r));
+Equations VFst {τ1 τ2 : Ty} (v : Value (TyPair τ1 τ2)) : Value τ1 :=
+  VFst (VPair x _) := x.
 
-  step (MkΣ (List (x :: xs)) ρ ANone κ) :=
-    MkΣ x ρ ANone (Fn (λ v, MkΣ (List xs) ρ (AList [v]) κ));
-  step (MkΣ (List (x :: xs)) ρ (AList r) κ) :=
-    MkΣ x ρ ANone (Fn (λ v, MkΣ (List xs) ρ (AList (v :: r)) κ));
+Equations VSnd {τ1 τ2 : Ty} (v : Value (TyPair τ1 τ2)) : Value τ2 :=
+  VSnd (VPair _ y) := y.
+
+Equations with_closure `(a : Exp Γ dom) (ρ : Env Γ) {τ} `(κ : Kont cod τ)
+          `(v : Value (dom ⟶ cod)) : Σ τ :=
+  with_closure a ρ κ (VClosure (Lambda e ρ')) :=
+    MkΣ a ρ (Fn (λ v, inl (MkΣ e (Val v ρ') κ))).
+
+Equations step {τ : Ty} (s : Σ τ) : Σ τ + Value τ :=
+  (* Constants *)
+  step (MkΣ (Constant x) _ (Fn f)) := f (VConst x);
+
+  step (MkΣ EUnit  _ (Fn f)) := f VUnit;
+  step (MkΣ ETrue  _ (Fn f)) := f VTrue;
+  step (MkΣ EFalse _ (Fn f)) := f VFalse;
+  step (MkΣ (If b t e) ρ κ) :=
+    inl (MkΣ b ρ (Fn (λ v, inl (MkΣ (IfBody t e v) ρ κ))));
+
+  step (MkΣ (Pair x y) ρ (Fn f)) :=
+    inl (MkΣ x ρ (Fn (λ v1, inl (MkΣ y ρ (Fn (λ v2, f (VPair v1 v2)))))));
+  step (MkΣ (Fst p) ρ (Fn f)) :=
+    inl (MkΣ p ρ (Fn (f ∘ VFst)));
+  step (MkΣ (Snd p) ρ (Fn f)) :=
+    inl (MkΣ p ρ (Fn (f ∘ VSnd)));
 
   (* A sequence just evaluates the second, for now *)
-  step (MkΣ (Seq e1 e2) ρ ANone κ) :=
-    MkΣ e2 ρ ANone κ;
+  step (MkΣ (Seq e1 e2) ρ κ) :=
+    inl (MkΣ e2 ρ κ);
 
   (* Let is a simple desugaring *)
-  step (MkΣ (Let x body) ρ ANone κ) :=
-    MkΣ (APP (LAM body) x) ρ ANone κ;
+  step (MkΣ (Let x body) ρ κ) :=
+    inl (MkΣ (APP (LAM body) x) ρ κ);
 
   (* A variable might lookup a lambda, in which case continue evaluating down
      that vein; otherwise, if no continuation, this is as far as we can go. *)
-  step (MkΣ (VAR v) ρ _ κ) with get ρ v := {
-    | VClosure (Lambda e ρ') => MkΣ (LAM e) ρ' ANone κ
+  step (MkΣ (VAR v) ρ κ) with get ρ v := {
+    | VClosure (Lambda e ρ') => inl (MkΣ (LAM e) ρ' κ)
     | x with κ := {
         | Fn f => f x
-        | Mt => MkΣ (VAR v) ρ ANone Mt
       }
   };
 
-  (* Lambda evaluates its argument, with the lambda as the cont *)
-  step (MkΣ (LAM e) ρ ANone (Ar a ρ' κ)) :=
-    MkΣ a ρ' ANone (Fn (λ v, MkΣ e (Val v ρ) ANone κ));
   (* If a lambda is passed, call it with the continuation *)
-  step (MkΣ (LAM e) ρ ANone (Fn f)) :=
+  step (MkΣ (LAM e) ρ (Fn f)) :=
     f (VClosure (Lambda e ρ));
 
   (* Application evaluates the lambda and then the argument *)
-  step (MkΣ (APP e1 e2) ρ ANone κ) :=
-    MkΣ e1 ρ ANone (Ar e2 ρ κ);
-
-  (* Otherwise, there is nothing more that can be done *)
-  step (MkΣ s ρ r Mt) := MkΣ s ρ r Mt.
+  step (MkΣ (APP e1 e2) ρ κ) :=
+    inl (MkΣ e1 ρ (Fn (inl ∘ with_closure e2 ρ κ))).
 
 Equations loop (gas : nat) {τ : Ty} (s : Σ τ) : Σ τ + Value τ :=
-  loop O s :=
-    inl s;
-  loop _ (MkΣ (Constant x) _ ANone Mt) :=
-    inr (VLit x);
-  loop _ (MkΣ (List []) _ ANone Mt) :=
-    inr (VList []);
-  loop _ (MkΣ (List []) _ (AList r) Mt) :=
-    inr (VList (rev r));
-  loop _ (MkΣ (VAR v) ρ ANone Mt) :=
-    inr (get ρ v);
-  loop (S gas') s :=
-    loop gas' (step s).
-
-Equations loop' (gas : nat) {τ : Ty} (s : Σ τ) : Σ τ :=
-  loop' O s := s;
-  loop' _ (MkΣ (Constant x) ρ r Mt) := MkΣ (Constant x) ρ r Mt;
-  loop' _ (MkΣ (List l)     ρ r Mt) := MkΣ (List l) ρ r Mt;
-  loop' _ (MkΣ (LAM e)      ρ r Mt) := MkΣ (LAM e) ρ r Mt;
-  loop' (S gas') s := loop' gas' (step s).
+  loop O s := inl s;
+  loop (S gas') s with step s := {
+    | inl s' => loop gas' s'
+    | inr r  => inr r
+  }.
 
 Definition run (gas : nat) {τ : Ty} {Γ : Exp.Env} (e : Exp Γ τ) (E : Env Γ) :
   Σ τ + Value τ := loop gas (inject e E).
 
 Example exp_constant :
-  run 10 (Constant (LInteger 123%Z)) Empty = inr (VLit (LInteger 123%Z)).
+  run 10 (Constant (LInteger 123%Z)) Empty = inr (VConst (LInteger 123%Z)).
 Proof. reflexivity. Qed.
 
-Example exp_list :
-  run 20 (List (Constant (LInteger 123%Z) ::
-                Constant (LInteger 456%Z) ::
-                Constant (LInteger 789%Z) :: [])) Empty =
-    inr (VList (VLit (LInteger 123%Z) ::
-                VLit (LInteger 456%Z) ::
-                VLit (LInteger 789%Z) :: [])).
+Example exp_pair :
+  run 20 (Pair (Constant (LInteger 123%Z))
+               (Constant (LInteger 456%Z))) Empty =
+    inr (VPair (VConst (LInteger 123%Z))
+               (VConst (LInteger 456%Z))).
 Proof. reflexivity. Qed.
 
 Example exp_let :
   run 10 (Let (Constant (LInteger 123%Z)) (VAR ZV)) Empty =
-    inr (VLit (LInteger 123%Z)).
+    inr (VConst (LInteger 123%Z)).
 Proof. reflexivity. Qed.
 
 Example exp_var :
-  run 10 (VAR ZV) (Val (VLit (LInteger 123%Z)) Empty) =
-    inr (VLit (LInteger 123%Z)).
+  run 10 (VAR ZV) (Val (VConst (LInteger 123%Z)) Empty) =
+    inr (VConst (LInteger 123%Z)).
 Proof. reflexivity. Qed.
 
 Example exp_lam τ :
   run 10 (LAM (cod:=τ) (VAR ZV)) Empty =
-    inl (MkΣ (LAM (VAR ZV)) Empty ANone Mt).
+    inr (VClosure (Lambda (VAR ZV) Empty)).
 Proof. reflexivity. Qed.
 
 Example exp_app :
   run 10 (APP (LAM (VAR ZV)) (Constant (LInteger 123%Z))) Empty =
-    inr (VLit (LInteger 123%Z)).
+    inr (VConst (LInteger 123%Z)).
 Proof. reflexivity. Qed.
 
-(*
-Theorem cek_sound τ (e : Exp [] τ) v :
-  e --->* v → ∃ gas, loop' gas (inject e Empty) = MkΣ v Empty ANone Mt.
+Theorem cek_sound τ (e : Exp [] τ) v v' :
+  e --->* v → represents [] v v' →
+  ∃ gas, loop gas (inject e Empty) = inr v'.
 Proof.
+  intros.
+  unfold inject.
+  induction H.
+  - dependent induction x;
+    exists 10%nat;
+    simp loop; simp step; simpl;
+    inv H0; auto.
+    + admit.
+    + now dependent elimination ρ.
+  - destruct IHmulti; auto.
+    induction H;
+    try solve [ exists (S x0);
+                simp loop; simp step; simpl;
+                rewrite <- H1; clear H1 ].
+    + exists (S (S x0)).
+      simp loop; simp step; simpl.
+      now simp loop; simp step; simpl.
+    + exists (S (S x0)).
+      simp loop; simp step; simpl.
+      now simp loop; simp step; simpl.
+    + exists x0.
 Abort.
-*)
 
 End CEK.
