src/Exp.v
@@ -19,10 +19,19 @@ Derive Signature NoConfusion for Var.
 
 Inductive Exp Γ : Ty → Type :=
   | Constant {ty} : Literal ty → Exp Γ (TyPrim ty)
+
+  | EUnit         : Exp Γ TyUnit
+
+  | ETrue         : Exp Γ TyBool
+  | EFalse        : Exp Γ TyBool
+  | If {τ}        : Exp Γ TyBool → Exp Γ τ → Exp Γ τ → Exp Γ τ
+
+  | Pair {τ1 τ2}  : Exp Γ τ1 → Exp Γ τ2 → Exp Γ (TyPair τ1 τ2)
+  | Fst {τ1 τ2}   : Exp Γ (TyPair τ1 τ2) → Exp Γ τ1
+  | Snd {τ1 τ2}   : Exp Γ (TyPair τ1 τ2) → Exp Γ τ2
+
   | Seq {τ τ'}    : Exp Γ τ' → Exp Γ τ → Exp Γ τ
-  (* The first list contains terms that need to be evaluated;
-     the second is a reversed list of terms in normal form. *)
-  | List {τ}      : list (Exp Γ τ) → Exp Γ (TyList τ)
+
   | Let {τ ty}    : Exp Γ ty → Exp (ty :: Γ) τ → Exp Γ τ
 
   (* These are the terms of the base lambda calculus *)
@@ -35,8 +44,14 @@ Derive Signature NoConfusionHom Subterm for Exp.
 Fixpoint Exp_size {Γ τ} (e : Exp Γ τ) : nat :=
   match e with
   | Constant _ x => 1
+  | EUnit _      => 1
+  | ETrue _      => 1
+  | EFalse _     => 1
+  | If _ b t e   => 1 + Exp_size b + Exp_size t + Exp_size e
+  | Pair _ x y   => 1 + Exp_size x + Exp_size y
+  | Fst _ p      => 1 + Exp_size p
+  | Snd _ p      => 1 + Exp_size p
   | Seq _ x y    => 1 + Exp_size x + Exp_size y
-  | List _ x     => 1 + fold_left plus (map Exp_size x) 0%nat
   | Let _ x body => 1 + Exp_size x + Exp_size body
   | VAR _ v      => 1
   | LAM _ e      => 1 + Exp_size e
@@ -45,70 +60,32 @@ Fixpoint Exp_size {Γ τ} (e : Exp Γ τ) : nat :=
 
 Corollary Exp_size_preserved {Γ τ} (e1 e2 : Exp Γ τ) :
   Exp_size e1 ≠ Exp_size e2 → e1 ≠ e2.
-Proof.
-  repeat intro; subst.
-  contradiction.
-Qed.
-
-Section Exp_rect.
-
-Variable P : ∀ Γ τ, Exp Γ τ → Type.
-
-Variable Pconstant : ∀ Γ ty (lit : Literal ty),
-  P Γ (TyPrim ty) (Constant Γ lit).
-Variable Pseq      : ∀ Γ τ τ' (e1 : Exp Γ τ') (e2 : Exp Γ τ),
-  P Γ τ' e1 → P Γ τ e2 → P Γ τ (Seq Γ e1 e2).
-Variable Plist     : ∀ Γ τ l,
-  ilist (P Γ τ) l → P Γ (TyList τ) (List Γ l).
-Variable Plet      : ∀ Γ τ ty (x : Exp Γ ty) (body : Exp (ty :: Γ) τ),
-  P Γ ty x →
-  P (ty :: Γ) τ body →
-  P Γ τ (Let _ x body).
-Variable Pvar      : ∀ Γ τ (v : Var Γ τ),
-  P Γ τ (VAR Γ v).
-Variable Plam      : ∀ Γ dom cod (e : Exp (dom :: Γ) cod),
-  P (dom :: Γ) cod e → P Γ (dom ⟶ cod) (LAM Γ e).
-Variable Papp      : ∀ Γ dom cod (e1 : Exp Γ (dom ⟶ cod)) (e2 : Exp Γ dom),
-  P Γ (dom ⟶ cod) e1 →
-  P Γ dom e2 →
-  P Γ cod (APP Γ e1 e2).
-
-Fixpoint Exp_rect' {Γ τ} (e : Exp Γ τ) : P Γ τ e.
-Proof.
-  induction e.
-  - now apply Pconstant.
-  - now apply Pseq.
-  - apply Plist.
-    induction l.
-    * exact tt.
-    * split.
-      ** now apply Exp_rect'.
-      ** exact IHl.
-  - now apply Plet.
-  - now apply Pvar.
-  - now apply Plam.
-  - now apply Papp.
-Qed.
-
-End Exp_rect.
+Proof. repeat intro; subst; contradiction. Qed.
 
 (* [ValueP] is an inductive proposition that indicates whether an expression
    represents a value, i.e., that it does reduce any further. *)
 Inductive ValueP Γ : ∀ {τ}, Exp Γ τ → Prop :=
   | ConstantP {ty} (l : Literal ty) :
     ValueP Γ (Constant Γ l)
-  | ListP {τ} (l : list (Exp Γ τ)) :
-    Forall (ValueP Γ) l →
-    ValueP Γ (List Γ l)
-  | ClosureP {dom cod} (e : Exp (dom :: Γ) cod) :
-    ValueP Γ (LAM Γ e).
+  | UnitP : ValueP Γ (EUnit Γ)
+  | TrueP : ValueP Γ (ETrue Γ)
+  | FalseP : ValueP Γ (EFalse Γ)
+  | PairP {τ1 τ2} {x : Exp Γ τ1} {y : Exp Γ τ2} :
+    ValueP Γ x → ValueP Γ y → ValueP Γ (Pair Γ x y)
+  | ClosureP {dom cod} (e : Exp (dom :: Γ) cod) : ValueP Γ (LAM Γ e).
 
 Arguments ZV {_ _}.
 Arguments SV {_ _ _} _.
 
 Arguments Constant {Γ ty} _.
+Arguments EUnit {Γ}.
+Arguments ETrue {Γ}.
+Arguments EFalse {Γ}.
+Arguments If {Γ τ} _ _ _.
+Arguments Pair {Γ τ1 τ2} _ _.
+Arguments Fst {Γ τ1 τ2} _.
+Arguments Snd {Γ τ1 τ2} _.
 Arguments Seq {Γ τ τ'} _ _.
-Arguments List {Γ τ} _.
 Arguments Let {Γ τ ty} _ _.
 Arguments VAR {Γ τ} _.
 Arguments LAM {Γ dom cod} _.
@@ -116,5 +93,8 @@ Arguments APP {Γ dom cod} _ _.
 
 Arguments ValueP {Γ τ} _.
 Arguments ConstantP {Γ ty} _.
-Arguments ListP {Γ τ} _.
+Arguments UnitP {Γ}.
+Arguments TrueP {Γ}.
+Arguments FalseP {Γ}.
+Arguments PairP {Γ τ1 τ2 x y} _ _.
 Arguments ClosureP {Γ dom cod} _.
